Casi SKIP ZER e INC per la dimostrazione di correttezza del compilatore LOOP -> SCORE

MasterThesis/LOOP/Language.lean
@@ -11,18 +11,18 @@ namespace store
 def emp : store := fun _ => 0
 
 def update (x : ident) (v : Nat) (s : store) : store :=
-  fun (y : ident) => if x == y then v else (s y)
+  fun (y : ident) => if x = y then v else (s y)
 
 notation "[" x " ↦ " v "]" s => update x v s -- Migliorare?
 notation "[" x " ↦ " v "]"   => [x ↦ v] emp -- Migliorare?
 
-theorem update_same (s : store) (x y : ident) (v : Nat) : x == y → (store.update x v s) y = v := by
+theorem update_same {s : store} {x y : ident} {v : Nat} : x = y → (store.update x v s) y = v := by
   intros
   unfold update
   apply if_pos
   assumption
 
-theorem update_other (s : store) (x y : ident) (v : Nat) : ¬(x == y) → (store.update x v s) y = (s y) := by
+theorem update_other {s : store} {x y : ident} {v : Nat} : x ≠ y → (store.update x v s) y = (s y) := by
   intros
   unfold update
   apply if_neg
